Fairness/PriceFairness.v
@@ -29,3 +29,20 @@ Proof.
   apply wf_state_execute_n.
   apply wf_state_initial.
 Qed.
+
+(* Price rule holds pointwise by definition of determine_clearing_price. *)
+Lemma price_rule_fairness_LTL_initial : forall bs as_list,
+  satisfies (mu_trace (initial_state bs as_list)) 0 (G (Atom p_price_rule)).
+Proof.
+  intros bs as_list.
+  rewrite satisfies_always_unfold.
+  intros j _.
+  rewrite mu_trace_atom_at_execute.
+  unfold interp_atom.
+  (* goal: price_rule_prop (execute j (initial_state bs as_list)) *)
+  unfold price_rule_prop.
+  destruct (marginal_pair (execute j (initial_state bs as_list))) as [[b a]|] eqn:Hmp; simpl; auto.
+  (* Unfold determine_clearing_price to normalize the equality. *)
+  unfold determine_clearing_price.
+  rewrite Hmp. reflexivity.
+Qed.
